

---

## Chapter 1. Foundations of Representation Theory

---

In this chapter we review four important module-theoretic theorems, which lie at the foundations of *representation theory of finite groups*:

1. **Schur's Lemma**: about homomorphisms between simple modules.
2. **The Jordan-Hölder Theorem**: about "uniqueness" properties of composition series.
3. **Nakayama's Lemma**: about an essential property of the Jacobson radical.
4. **The Krull-Schmidt Theorem**: about direct sum decompositions into indecomposable submodules.

**Notation**: throughout this chapter, unless otherwise specified, we let  $R$  denote an arbitrary unital and associative ring.

Again results which intersect the *Commutative Algebra* lecture are stated without proof.

### References:

- [CR90] C. W. CURTIS AND I. REINER, *Methods of representation theory. Vol. I*, Wiley Classics Library, John Wiley & Sons, Inc., New York, 1990.
- [Dor72] L. DORNHOFF, *Group representation theory. Part B: Modular representation theory*, Marcel Dekker, Inc., New York, 1972.
- [NT89] H. NAGAO AND Y. TSUSHIMA, *Representations of finite groups*, Translated from the Japanese. Academic Press, Inc., Boston, MA, 1989.
- [Rot10] J. J. ROTMAN, *Advanced modern algebra. 2nd ed.*, Providence, RI: American Mathematical Society (AMS), 2010.

## 6 (Ir)Reducibility and (in)decomposability

Submodules and direct sums of modules allow us to introduce the two main notions that will enable us to break modules in *elementary* pieces in order to simplify their study.

**Definition 6.1 (simple/irreducible module / indecomposable module)**

- (a) An  $R$ -module  $M$  is called **reducible** if it admits an  $R$ -submodule  $U$  such that  $0 \subsetneq U \subsetneq M$ .  
An  $R$ -module  $M$  is called **simple** (or **irreducible**) if it is non-zero and not reducible.
- (b) An  $R$ -module  $M$  is called **decomposable** if  $M$  possesses two non-zero proper submodules  $M_1, M_2$  such that  $M = M_1 \oplus M_2$ . An  $R$ -module  $M$  is called **indecomposable** if it is non-zero and not decomposable.

**Remark 6.2**

Clearly any simple module is also indecomposable. However, the converse does not hold in general.  
Exercise: find a counter-example!

**Exercise 6.3**

Prove that if  $(R, +, \cdot)$  is a ring, then  $R^\circ := R$  itself may be seen as an  $R$ -module via left multiplication in  $R$ , i.e. where the external composition law is given by

$$R \times R^\circ \longrightarrow R^\circ, (r, m) \mapsto r \cdot m.$$

We call  $R^\circ$  the **regular**  $R$ -module.

Prove that the  $R$ -submodules of  $R^\circ$  are precisely the left ideals of  $R$ . Moreover,  $I \triangleleft R$  is a maximal left ideal of  $R \Leftrightarrow R^\circ/I$  is a simple  $R$ -module, and  $I \triangleleft R$  is a minimal left ideal of  $R \Leftrightarrow I$  is simple when regarded as an  $R$ -submodule of  $R^\circ$ .

## 7 Schur's Lemma

Schur's Lemma is a basic result, which lets us understand homomorphisms between *simple* modules, and, more importantly, endomorphisms of such modules.

**Theorem 7.1 (Schur's Lemma)**

- (a) Let  $V, W$  be simple  $R$ -modules. Then:
- (i)  $\text{End}_R(V)$  is a skew-field, and
  - (ii) if  $V \not\cong W$ , then  $\text{Hom}_R(V, W) = 0$ .
- (b) If  $K$  is an algebraically closed field,  $A$  is a  $K$ -algebra, and  $V$  is a simple  $A$ -module such that  $\dim_K V < \infty$ , then

$$\text{End}_A(V) = \{\lambda \text{Id}_V \mid \lambda \in K\} \cong K.$$

**Proof:**

- (a) First, we claim that every  $f \in \text{Hom}_R(V, W) \setminus \{0\}$  admits an inverse in  $\text{Hom}_R(V, W)$ .  
Indeed,  $f \neq 0 \implies \ker f \subsetneq V$  is a proper  $R$ -submodule of  $V$  and  $\{0\} \neq \text{Im } f$  is a non-zero  $R$ -submodule of  $W$ . But then, on the one hand,  $\ker f = \{0\}$ , because  $V$  is simple, hence  $f$  is injective, and on the other hand,  $\text{Im } f = W$  because  $W$  is simple. It follows that  $f$  is also surjective, hence

bijjective. Therefore, by Example 1(d),  $f$  is invertible with inverse  $f^{-1} \in \text{Hom}_R(V, W)$ .

Now, (ii) is straightforward from the above. For (i), by Exercise 2.2,  $\text{End}_R(V)$  is a ring, which is obviously non-zero as  $\text{End}_R(V) \ni \text{Id}_V$  and  $\text{Id}_V \neq 0$  because  $V \neq 0$  since it is simple. Thus, as any  $f \in \text{End}_R(V) \setminus \{0\}$  is invertible,  $\text{End}_R(V)$  is a skew-field.

- (b) Let  $f \in \text{End}_A(V)$ . By the assumptions on  $K$ ,  $f$  has an eigenvalue  $\lambda \in K$ . Let  $v \in V \setminus \{0\}$  be an eigenvector of  $f$  for  $\lambda$ . Then  $(f - \lambda \text{Id}_V)(v) = 0$ . Therefore,  $f - \lambda \text{Id}_V$  is not invertible and

$$f - \lambda \text{Id}_V \in \text{End}_A(V) \xrightarrow{(a)} f - \lambda \text{Id}_V = 0 \implies f = \lambda \text{Id}_V.$$

Hence  $\text{End}_A(V) \subseteq \{\lambda \text{Id}_V \mid \lambda \in K\}$ , but the reverse inclusion also obviously holds, so that

$$\text{End}_A(V) = \{\lambda \text{Id}_V\} \cong K.$$

■

## 8 Composition series and the Jordan-Hölder Theorem\*

From Chapter 2 on, we will assume that all modules we work with can be broken into *simple* modules in the sense of the following definition.

### Definition 8.1 (Composition series / composition factors / composition length)

Let  $M$  be an  $R$ -module.

- (a) A **series** (or **filtration**) of  $M$  is a finite chain of submodules

$$0 = M_0 \subseteq M_1 \subseteq \dots \subseteq M_n = M \quad (n \in \mathbb{Z}_{\geq 0}).$$

- (b) A **composition series** of  $M$  is a series

$$0 = M_0 \subseteq M_1 \subseteq \dots \subseteq M_n = M \quad (n \in \mathbb{Z}_{\geq 0})$$

where  $M_i/M_{i-1}$  is simple for each  $1 \leq i \leq n$ . The quotient modules  $M_i/M_{i-1}$  are called the **composition factors** (or the **constituents**) of  $M$  and the integer  $n$  is called the **composition length** of  $M$ .

Notice that, clearly, in a composition series all inclusions are in fact strict because the quotient modules are required to be simple, hence non-zero.

Next we see that the existence of a *composition series* implies that the module is *finitely generated*. However, the converse does not hold in general. This is explained through the fact that the existence of a composition series is equivalent to the fact that the module is both *Noetherian* and *Artinian*.

### Definition 8.2 (Chain conditions / Artinian and Noetherian rings and modules)

- (a) An  $R$ -module  $M$  is said to satisfy the **descending chain condition** (D.C.C.) on submodules (or to be **Artinian**) if every descending chain  $M = M_0 \supseteq M_1 \supseteq \dots \supseteq M_r \supseteq \dots \supseteq \{0\}$  of

submodules eventually becomes stationary, i.e.  $\exists m_0$  such that  $M_m = M_{m_0}$  for every  $m \geq m_0$ .

- (b) An  $R$ -module  $M$  is said to satisfy the **ascending chain condition** (A.C.C.) on submodules (or to be **Noetherian**) if every ascending chain  $0 = M_0 \subseteq M_1 \subseteq \dots \subseteq M_r \subseteq \dots \subseteq M$  of submodules eventually becomes stationary, i.e.  $\exists m_0$  such that  $M_m = M_{m_0}$  for every  $m \geq m_0$ .
- (c) The ring  $R$  is called **left Artinian** (resp. **left Noetherian**) if the regular module  $R^\circ$  is Artinian (resp. Noetherian).

### Theorem 8.3 (Jordan-Hölder)

Any series of  $R$ -submodules  $0 = M_0 \subseteq M_1 \subseteq \dots \subseteq M_r = M$  ( $r \in \mathbb{Z}_{\geq 0}$ ) of an  $R$ -module  $M$  may be refined to a composition series of  $M$ . In addition, if

$$0 = M_0 \subsetneq M_1 \subsetneq \dots \subsetneq M_n = M \quad (n \in \mathbb{Z}_{\geq 0})$$

and

$$0 = M'_0 \subsetneq M'_1 \subsetneq \dots \subsetneq M'_m = M \quad (m \in \mathbb{Z}_{\geq 0})$$

are two composition series of  $M$ , then  $m = n$  and there exists a permutation  $\pi \in \mathfrak{S}_n$  such that  $M'_i/M'_{i-1} \cong M_{\pi(i)}/M_{\pi(i)-1}$  for every  $1 \leq i \leq n$ . In particular, the composition length is well-defined.

**Proof:** See *Commutative Algebra*. ■

### Corollary 8.4

If  $M$  is an  $R$ -module, then TFAE:

- (a)  $M$  has a composition series;
- (b)  $M$  satisfies D.C.C. and A.C.C. on submodules;
- (c)  $M$  satisfies D.C.C. on submodules and every submodule of  $M$  is finitely generated.

**Proof:** See *Commutative Algebra*. ■

### Theorem 8.5 (Hopkins' Theorem)

If  $M$  is a module over a left Artinian ring, then TFAE:

- (a)  $M$  has a composition series;
- (b)  $M$  satisfies D.C.C. on submodules;
- (c)  $M$  satisfies A.C.C. on submodules;
- (d)  $M$  is finitely generated.

**Proof:** See *Commutative Algebra*. (Or [Exercise](#): deduce it from the properties of the Jacobson radical and semisimplicity, which we are going to develop in the next sections.) ■

## 9 The Jacobson radical and Nakayama's Lemma\*

The Jacobson radical is one of the most important two-sided ideals of a ring. As we will see in the next sections and Chapter 2, this ideal carries a lot of information about the structure of a ring and that of its modules.

### Proposition-Definition 9.1 (*Annihilator / Jacobson radical*)

(a) Let  $M$  be an  $R$ -module. Then  $\text{ann}_R(M) := \{r \in R \mid rm = 0 \ \forall m \in M\}$  is a two-sided ideal of  $R$ , called **annihilator** of  $M$ .

(b) The **Jacobson radical** of  $R$  is the two-sided ideal

$$J(R) := \bigcap_{\substack{V \text{ simple} \\ R\text{-module}}} \text{ann}_R(V) = \{x \in R \mid 1 - axb \in R^\times \ \forall a, b \in R\}.$$

(c) If  $V$  is a simple  $R$ -module, then there exists a maximal left ideal  $I \triangleleft R$  such that  $V \cong R^\circ/I$  (as  $R$ -modules) and

$$J(R) = \bigcap_{\substack{I \triangleleft R, \\ I \text{ maximal} \\ \text{left ideal}}} I.$$

**Proof:** See *Commutative Algebra*. ■

### Exercise 9.2

- (a) Prove that any simple  $R$ -module may be seen as a simple  $R/J(R)$ -module.
- (b) Conversely, prove that any simple  $R/J(R)$ -module may be seen as a simple  $R$ -module. [Hint: use a change of the base ring via the canonical morphism  $R \rightarrow R/J(R)$ .]
- (c) Deduce that  $R$  and  $R/J(R)$  have the same simple modules.

### Theorem 9.3 (*Nakayama's Lemma*)

If  $M$  is a finitely generated  $R$ -module and  $J(R)M = M$ , then  $M = 0$ .

**Proof:** See *Commutative Algebra*. ■

### Remark 9.4

One often needs to apply Nakayama's Lemma to a finitely generated quotient module  $M/U$ , where  $U$  is an  $R$ -submodule of  $M$ . In that case the result may be restated as follows:

$$M = U + J(R)M \implies U = M$$

## 10 Indecomposability and the Krull-Schmidt Theorem

We now consider the notion of *indecomposability* in more details. Our first aim is to prove that indecomposability can be recognised at the endomorphism algebra of a module.

### Definition 10.1

A ring  $R$  is said to be **local**  $\iff R \setminus R^\times$  is a two-sided ideal of  $R$ .

### Example 5

- (a) Any field  $K$  is local because  $K \setminus K^\times = \{0\}$  by definition.
- (b) Exercise: Let  $p$  is a prime number and  $R := \{\frac{a}{b} \in \mathbb{Q} \mid p \nmid b\}$ . Prove that  $R \setminus R^\times = \{\frac{a}{b} \in R \mid p \mid a\}$  and deduce that  $R$  is local.
- (c) Exercise: Let  $K$  be a field and let  $R := \left\{ A = \begin{pmatrix} a_1 & a_2 & \dots & a_n \\ 0 & a_1 & \dots & a_{n-1} \\ \vdots & \ddots & \ddots & \vdots \\ 0 & 0 & \dots & a_1 \end{pmatrix} \in M_n(K) \right\}$ . Prove that  $R \setminus R^\times = \{A \in R \mid a_1 = 0\}$  and deduce that  $R$  is local.

### Proposition 10.2

Let  $R$  be a ring. Then TFAE:

- (a)  $R$  is local;
- (b)  $R \setminus R^\times = J(R)$ , i.e.  $J(R)$  is the unique maximal left ideal of  $R$ ;
- (c)  $R/J(R)$  is a skew-field.

**Proof:** Set  $N := R \setminus R^\times$ .

(a) $\Rightarrow$ (b): Clear:  $I \triangleleft R$  proper left ideal  $\Rightarrow I \subseteq N$ . Hence, by Proposition-Definition 9.1(c),

$$J(R) = \bigcap_{\substack{I \triangleleft R, \\ I \text{ maximal} \\ \text{left ideal}}} I \subseteq N.$$

Now, by (a)  $N$  is an ideal of  $R$ , hence  $N$  must be a maximal left ideal, even the unique one. It follows that  $N = J(R)$ .

(b) $\Rightarrow$ (c): If  $J(R)$  is the unique maximal left ideal of  $R$ , then in particular  $R \neq 0$  and  $R/J(R) \neq 0$ . So let  $r \in R \setminus J(R) \stackrel{(b)}{=} R^\times$ . Then obviously  $r + J(R) \in (R/J(R))^\times$ . It follows that  $R/J(R)$  is a skew-field.

(c) $\Rightarrow$ (a): Since  $R/J(R)$  is a skew-field by (c),  $R/J(R) \neq 0$ , so that  $R \neq 0$  and there exists  $a \in R \setminus J(R)$ . Moreover, again by (c),  $a + J(R) \in (R/J(R))^\times$ , so that  $\exists b \in R \setminus J(R)$  such that

$$ab + J(R) = 1 + J(R) \in R/J(R)$$

Therefore,  $\exists c \in J(R)$  such that  $ab = 1 - c$ , which is invertible in  $R$  by Proposition-Definition 9.1(b). Hence  $\exists d \in R$  such that  $abd = (1 - c)d = 1 \Rightarrow a \in R^\times$ . Therefore  $R \setminus J(R) = R^\times$ , and it follows that  $R \setminus R^\times = J(R)$  which is a two-sided ideal of  $R$ . ■

**Proposition 10.3 (Fitting's Lemma)**

Let  $M$  be an  $R$ -module which has a composition series and let  $\varphi \in \text{End}_R(M)$  be an endomorphism of  $M$ . Then there exists  $n \in \mathbb{Z}_{>0}$  such that

- (i)  $\varphi^n(M) = \varphi^{n+i}(M)$  for every  $i \geq 1$ ;
- (ii)  $\ker(\varphi^n) = \ker(\varphi^{n+i})$  for every  $i \geq 1$ ; and
- (iii)  $M = \varphi^n(M) \oplus \ker(\varphi^n)$ .

**Proof:** By Corollary 8.4 the module  $M$  satisfies both A.C.C. and D.C.C. on submodules. Hence the two chains of submodules

$$\varphi(M) \supseteq \varphi^2(M) \supseteq \dots,$$

$$\ker(\varphi) \subseteq \ker(\varphi^2) \subseteq \dots$$

eventually become stationary. Therefore we can find an index  $n$  satisfying both (i) and (ii).

**Exercise:** Prove that  $M = \varphi^n(M) \oplus \ker(\varphi^n)$ . ■

**Proposition 10.4**

Let  $M$  be an  $R$ -module which has a composition series. Then:

$$M \text{ is indecomposable} \iff \text{End}_R(M) \text{ is a local ring.}$$

**Proof:** " $\Rightarrow$ ": Assume that  $M$  is indecomposable. Let  $\varphi \in \text{End}_R(M)$ . Then by Fitting's Lemma there exists  $n \in \mathbb{Z}_{>0}$  such that  $M = \varphi^n(M) \oplus \ker(\varphi^n)$ . As  $M$  is indecomposable either  $\varphi^n(M) = M$  and  $\ker(\varphi^n) = 0$  or  $\varphi^n(M) = 0$  and  $\ker(\varphi^n) = M$ .

- In the first case  $\varphi$  is bijective, hence invertible.
- In the second case  $\varphi$  is nilpotent.

Therefore,  $N := \text{End}_R(M) \setminus \text{End}_R(M)^\times = \{\text{nilpotent elements of } \text{End}_R(M)\}$ .

**Claim:**  $N$  is a two-sided ideal of  $\text{End}_R(M)$ .

Let  $\varphi \in N$  and  $m \in \mathbb{Z}_{>0}$  minimal such that  $\varphi^m = 0$ . Then

$$\varphi^{m-1}(\varphi\rho) = 0 = (\rho\varphi)\varphi^{m-1} \quad \forall \rho \in \text{End}_R(M).$$

As  $\varphi^{m-1} \neq 0$ ,  $\varphi\rho$  and  $\rho\varphi$  cannot be invertible, hence  $\varphi\rho, \rho\varphi \in N$ .

Next let  $\varphi, \rho \in N$ . If  $\varphi + \rho =: \psi$  were invertible in  $\text{End}_R(M)$ , then by the previous argument we would have  $\psi^{-1}\rho, \psi^{-1}\varphi \in N$ , which would be nilpotent. Hence

$$\psi^{-1}\varphi = \text{Id}_M - \psi^{-1}\rho$$

would be invertible.

(Indeed,  $\psi^{-1}\rho$  nilpotent  $\Rightarrow (\text{Id}_M - \psi^{-1}\rho)(\text{Id}_M + \psi^{-1}\rho + (\psi^{-1}\rho)^2 + \dots + (\psi^{-1}\rho)^{a-1}) = \text{Id}_M$ , where  $a$  is minimal such that  $(\psi^{-1}\rho)^a = 0$ .)

This is a contradiction. Therefore  $\varphi + \rho \in N$ , which proves that  $N$  is an ideal.

Finally, it follows from the Claim and the definition that  $\text{End}_R(M)$  is local.

" $\Leftarrow$ ": Assume  $M$  is decomposable and let  $M_1, M_2$  be proper submodules such that  $M = M_1 \oplus M_2$ . Then consider the two projections

$$\pi_1 : M_1 \oplus M_2 \longrightarrow M_1 \oplus M_2, (m_1, m_2) \mapsto (m_1, 0)$$

onto  $M_1$  along  $M_2$  and

$$\pi_2 : M_1 \oplus M_2 \longrightarrow M_1 \oplus M_2, (m_1, m_2) \mapsto (0, m_2)$$

onto  $M_2$  along  $M_1$ . Clearly  $\pi_1, \pi_2 \in \text{End}_R(M)$  but  $\pi_1, \pi_2 \notin \text{End}_R(M)^\times$  since they are not surjective by construction. Now, as  $\pi_2 = \text{Id}_M - \pi_1$  is not invertible it follows from the characterisation of the Jacobson radical of Proposition-Definition 9.1(b) that  $\pi_1 \notin J(\text{End}_R(M))$ . Therefore

$$\text{End}_R(M) \setminus \text{End}_R(M)^\times \neq J(\text{End}_R(M))$$

and it follows from Proposition 10.2 that  $\text{End}_R(M)$  is not a local ring. ■

Next, we want to be able to decompose  $R$ -modules into direct sums of indecomposable submodules. The Krull-Schmidt Theorem will then provide us with certain uniqueness properties of such decompositions.

### Proposition 10.5

Let  $M$  be an  $R$ -module. If  $M$  satisfies either A.C.C. or D.C.C., then  $M$  admits a decomposition into a direct sum of finitely many indecomposable  $R$ -submodules.

**Proof:** Let us assume that  $M$  is not expressible as a finite direct sum of indecomposable submodules. Then in particular  $M$  is decomposable, so that we may write  $M = M_1 \oplus W_1$  as a direct sum of two proper submodules. W.l.o.g. we may assume that the statement is also false for  $W_1$ . Then we also have a decomposition  $W_1 = M_2 \oplus W_2$ , where  $M_2$  and  $W_2$  are proper submodules of  $W_1$  with the statement being false for  $W_2$ . Iterating this argument yields the following infinite chains of submodules:

$$W_1 \supsetneq W_2 \supsetneq W_3 \supsetneq \dots,$$

$$M_1 \subsetneq M_1 \oplus M_2 \subsetneq M_1 \oplus M_2 \oplus M_3 \subsetneq \dots.$$

The first chain contradicts D.C.C. and the second chain contradicts A.C.C.. The claim follows. ■

### Theorem 10.6 (Krull-Schmidt)

Let  $M$  be an  $R$ -module which has a composition series. If

$$M = M_1 \oplus \dots \oplus M_n = M'_1 \oplus \dots \oplus M'_{n'}, \quad (n, n' \in \mathbb{Z}_{>0})$$

are two decomposition of  $M$  into direct sums of finitely many indecomposable  $R$ -submodules, then  $n = n'$ , and there exists a permutation  $\pi \in \mathfrak{S}_n$  such that  $M_i \cong M'_{\pi(i)}$  for each  $1 \leq i \leq n$  and

$$M = M'_{\pi(1)} \oplus \dots \oplus M'_{\pi(r)} \oplus \bigoplus_{j=r+1}^n M_j \quad \text{for every } 1 \leq r \leq n.$$

**Proof:** For each  $1 \leq i \leq n$  let

$$\pi_i : M = M_1 \oplus \dots \oplus M_n \rightarrow M_i, m_1 + \dots + m_n \mapsto m_i$$

be the projection on the  $i$ -th factor of first decomposition, and for each  $1 \leq j \leq n'$  let

$$\psi_j : M = M'_1 \oplus \dots \oplus M'_{n'} \rightarrow M'_j, m'_1 + \dots + m'_{n'} \mapsto m'_j$$

be the projection on the  $j$ -th factor of second decomposition.



**Claim:** if  $\psi \in \text{End}_R(M)$  is such that  $\pi_1 \circ \psi|_{M_1} : M_1 \rightarrow M_1$  is an isomorphism, then

$$M = \psi(M_1) \oplus M_2 \oplus \cdots \oplus M_n \text{ and } \psi(M_1) \cong M_1.$$

*Indeed:* By the assumption of the claim, both  $\psi|_{M_1} : M_1 \rightarrow \psi(M_1)$  and  $\pi_1|_{\psi(M_1)} : \psi(M_1) \rightarrow M_1$  must be isomorphisms. Therefore  $\psi(M_1) \cap \ker(\pi_1) = 0$ , and for every  $m \in M$  there exists  $m'_1 \in \psi(M_1)$  such that  $\pi_1(m) = \pi_1(m'_1)$ , hence  $m - m'_1 \in \ker(\pi_1)$ . It follows that

$$M = \psi(M_1) + \ker(\pi_1) = \psi(M_1) \oplus \ker(\pi_1) = \psi(M_1) \oplus M_2 \oplus \cdots \oplus M_n.$$

Hence the Claim holds.

Now, we have  $\text{Id}_M = \sum_{j=1}^{n'} \psi_j$ , and so  $\text{Id}_{M_1} = \sum_{j=1}^{n'} \pi_1 \circ \psi_j|_{M_1} \in \text{End}_R(M_1)$ . But as  $M$  has a composition series, so has  $M_1$ , and therefore  $\text{End}_R(M_1)$  is local by Proposition 10.4. Thus if all the  $\pi_1 \circ \psi_j|_{M_1} \in \text{End}_R(M_1)$  are not invertible, they are all nilpotent and then so is  $\text{Id}_{M_1}$ , which is in turn not invertible. This is not possible, hence it follows that there exists an index  $j$  such that

$$\pi_1 \circ \psi_j|_{M_1} : M_1 \rightarrow M_1$$

is an isomorphism and the Claim implies that  $M = \psi_j(M_1) \oplus M_2 \oplus \cdots \oplus M_n$  and  $\psi_j(M_1) \cong M_1$ . We then set  $\pi(1) := j$ . By definition  $\psi_j(M_1) \subseteq M'_j$  as  $M'_j$  is indecomposable, so that

$$\psi_j(M_1) \cong M'_j = M'_{\pi(1)}.$$

Finally, an induction argument ([Exercise!](#)) yields:

$$M = M'_{\pi(1)} \oplus \cdots \oplus M'_{\pi(r)} \oplus \bigoplus_{j=r+1}^n M_j,$$

mit  $M'_{\pi(i)} \cong M_i$  ( $1 \leq i \leq r$ ). In particular, the case  $r = n$  implies the equality  $n = n'$ . ■